Makefile
@@ -12,6 +12,11 @@ coq:
 	coqc -R . "" Trace.v
 	coqc -R . "" Machine.v
 	coqc -R . "" ObsTrace.v
+	coqc -R . "" SubroutineSimple.v
+	coqc -R . "" TraceProperties.v
+	coqc -R . "" SubroutineShare.v
+	coqc -R . "" Coroutine.v
+	coqc -R . "" Lazy.v
 
 clean:
 	rm -f *.aux *.vio *.vo* *.glob
